AwsCryptographicMaterialProviders/dafny/AwsCryptographicMaterialProviders/src/Keyrings/AwsKms/AwsKmsRsaKeyring.dfy
@@ -109,8 +109,29 @@ module AwsKmsRsaKeyring {
       this.grantTokens := grantTokens;
     }
 
-    predicate OnEncryptEnsuresPublicly(input: Types.OnEncryptInput , output: Result<Types.OnEncryptOutput, Types.Error>)
-    {true}
+    predicate OnEncryptEnsuresPublicly (
+      input: Types.OnEncryptInput ,
+      output: Result<Types.OnEncryptOutput, Types.Error> )
+      : (outcome: bool)
+      ensures
+        outcome ==>
+          output.Success?
+          ==>
+            && Materials.EncryptionMaterialsHasPlaintextDataKey(output.value.materials)
+            && Materials.ValidEncryptionMaterialsTransition(
+                 input.materials,
+                 output.value.materials
+               )
+    {
+      output.Success?
+      ==>
+        && Materials.EncryptionMaterialsHasPlaintextDataKey(output.value.materials)
+        && Materials.ValidEncryptionMaterialsTransition(
+             input.materials,
+             output.value.materials
+           )
+    }
+
 
     method OnEncrypt'(input: Types.OnEncryptInput)
       returns (res: Result<Types.OnEncryptOutput, Types.Error>)
@@ -185,7 +206,24 @@ module AwsKmsRsaKeyring {
       return Success(Types.OnEncryptOutput(materials := returnMaterials));
     }
 
-    predicate OnDecryptEnsuresPublicly ( input: Types.OnDecryptInput , output: Result<Types.OnDecryptOutput, Types.Error> ) {true}
+    predicate OnDecryptEnsuresPublicly ( input: Types.OnDecryptInput , output: Result<Types.OnDecryptOutput, Types.Error> )
+      : (outcome: bool)
+      ensures
+        outcome ==>
+          output.Success?
+          ==>
+            && Materials.DecryptionMaterialsTransitionIsValid(
+              input.materials,
+              output.value.materials
+            )
+    {
+      output.Success?
+      ==>
+        && Materials.DecryptionMaterialsTransitionIsValid(
+          input.materials,
+          output.value.materials
+        )
+    }
 
     method OnDecrypt'(input: Types.OnDecryptInput)
       returns (res: Result<Types.OnDecryptOutput, Types.Error>)
@@ -382,6 +420,10 @@ module AwsKmsRsaKeyring {
         && Seq.Last(client.History.Decrypt).output.value.KeyId == Some(awsKmsKey)
     }
 
+    predicate Requires(edk: Types.EncryptedDataKey){
+      true
+    }
+
     method Invoke(
       edk: Types.EncryptedDataKey,
       ghost attemptsState: seq<ActionInvoke<Types.EncryptedDataKey, Result<Materials.SealedDecryptionMaterials, Types.Error>>>
@@ -482,7 +524,8 @@ module AwsKmsRsaKeyring {
         MaterialWrapping.WrapInput(
           plaintextMaterial := plaintextMaterial,
           algorithmSuite := input.algorithmSuite,
-          encryptionContext := input.encryptionContext
+          encryptionContext := input.encryptionContext,
+          serializedEC := input.serializedEC
         ), []);
 
       var output := MaterialWrapping.GenerateAndWrapOutput(
