StandardLibrary/src/Sequence.dfy
@@ -2,10 +2,50 @@
 // SPDX-License-Identifier: Apache-2.0
 
 include "UInt.dfy"
+include "WrappersInterop.dfy"
 
 module StandardLibrary.Sequence {
   // export provides SequenceEqual, StandardLibrary
   import opened UInt
+  import opened Wrappers
+
+  // Just like Seq::MapWithResult, but not O(n^2)
+  function method {:opaque} {:tailrecursion} MapWithResult<T, R, E>(f: (T ~> Result<R, E>), xs: seq<T>, pos : nat := 0, acc : seq<R> := [])
+    : (result: Result<seq<R>, E>)
+    requires forall i :: 0 <= i < |xs| ==> f.requires(xs[i])
+    requires pos <= |xs|
+    requires |acc| == pos
+    requires forall i :: 0 <= i < pos ==>
+                           && f(xs[i]).Success?
+                           && acc[i] == f(xs[i]).value
+
+    ensures result.Success? ==>
+              && |result.value| == |xs|
+              && (forall i :: 0 <= i < |xs| ==>
+                                && f(xs[i]).Success?
+                                && result.value[i] == f(xs[i]).value)
+    reads set i, o | 0 <= i < |xs| && o in f.reads(xs[i]) :: o
+    decreases |xs| - pos
+  {
+    if |xs| == pos then
+      Success(acc)
+    else
+      var head :- f(xs[pos]);
+      MapWithResult(f, xs, pos+1, acc + [head])
+  }
+
+
+  /* Flattens a sequence of sequences into a single sequence by concatenating 
+     subsequences, starting from the first element. */
+  function method {:tailrecursion} Flatten<T>(xs: seq<seq<T>>, pos : nat := 0, acc : seq<T> := []): (ret : seq<T>)
+    requires pos <= |xs|
+    decreases |xs| - pos
+  {
+    if |xs| == pos then
+      acc
+    else
+      Flatten(xs, pos+1, acc + xs[pos])
+  }
 
   predicate method SequenceEqualNat<T(==)>(seq1: seq<T>, seq2: seq<T>, start1: nat, start2: nat, size: nat) : (ret : bool)
     requires start1 + size <= |seq1|
